@prefix write: <https://wendang-project.github.io/ontology/> .
@prefix wd: <http://www.wikidata.org/entity/> .
@prefix wdt: <http://www.wikidata.org/prop/> .
@prefix owl: <http://www.w3.org/2002/07/owl#> .
@prefix rdf: <http://www.w3.org/1999/02/22-rdf-syntax-ns#> .
@prefix xml: <http://www.w3.org/XML/1998/namespace> .
@prefix xsd: <http://www.w3.org/2001/XMLSchema#> .
@prefix rdfs: <http://www.w3.org/2000/01/rdf-schema#> .
@prefix skos: <http://www.w3.org/2004/02/skos/core#> .
@prefix dcterms: <http://purl.org/dc/terms/> .

<https://wendang-project.github.io/ontology/> rdf:type owl:Ontology ;
                                               owl:versionIRI write:v1.0.0 ;
                                               dcterms:creator "Katarina Lučić" ;
                                               dcterms:license "This work is licensed under the Creative Commons Attribution 4.0 International License (https://creativecommons.org/licenses/by/4.0/)." ;
                                               dcterms:modified "2025-02-05T00:00:00" ;
                                               dcterms:subject "\"Chinese calligraphy\", \"contemporary calligraphy\", \"contemporary arts\", \"visual arts\", \"graffiti\", \"performing art\", \"decorative and applied arts\"" ;
                                               dcterms:version "1.0.0" ;
                                               rdfs:comment "This ontology is designed to represent the intangible cultural heritage of Chinese calligraphy as it appears in contemporary artworks, alongside the broader tangible cultural heritage of contemporary arts. The WRITE ontology provides a structured way to describe artworks, their contextual elements, and the calligraphy integrated within them. Additionally, it facilitates the identification of similarities and differences between contemporary and traditional calligraphy, enabling a deeper understanding of their evolution and artistic connections." ,
                                                            "This ontology was developed with input from domain experts, all of whom are members of the WRITE project team. To learn more about the project, please visit: https://writecalligraphyproject.eu/." ;
                                               rdfs:label "WRITE ontology" ;
                                               dcterms:contributor "Valentina Pasqual (former contributor)" .

#################################################################
#    Annotation properties
#################################################################

###  http://purl.org/dc/terms/contributor
dcterms:contributor rdf:type owl:AnnotationProperty .


###  http://purl.org/dc/terms/creator
dcterms:creator rdf:type owl:AnnotationProperty .


###  http://purl.org/dc/terms/license
dcterms:license rdf:type owl:AnnotationProperty .


###  http://purl.org/dc/terms/modified
dcterms:modified rdf:type owl:AnnotationProperty .


###  http://purl.org/dc/terms/subject
dcterms:subject rdf:type owl:AnnotationProperty .


###  http://purl.org/dc/terms/version
dcterms:version rdf:type owl:AnnotationProperty .


#################################################################
#    Datatypes
#################################################################

###  http://www.w3.org/2001/XMLSchema#date
xsd:date rdf:type rdfs:Datatype .


###  http://www.w3.org/2001/XMLSchema#duration
xsd:duration rdf:type rdfs:Datatype .


#################################################################
#    Object Properties
#################################################################

###  http://www.wikidata.org/prop/P749
wdt:P749 rdf:type owl:ObjectProperty ;
         rdfs:domain wd:Q43229 ;
         rdfs:range wd:Q43229 ;
         rdfs:comment "Indicates a close relation between two organisations (e.g., research centre and university)." ;
         rdfs:label "affiliated to" .


###  http://www.wikidata.org/prop/P84
wdt:P84 rdf:type owl:ObjectProperty ;
        rdfs:domain write:DecorativeAndAppliedArt ;
        rdfs:range wd:Q1400264 ,
                   wd:Q215627 ;
        rdfs:comment "Architect or architectural firm responsible for designing a building or other structure." ;
        rdfs:label "architect" .

###  https://wendang-project.github.io/ontology/artistic-collective-type
write:artistic-collective-type rdf:type owl:ObjectProperty ;
                               rdfs:domain wd:Q1400264 ;
                               rdfs:range owl:Thing ;
                               rdfs:comment "Indicates the type of artistic collective (e.g., graffiti crew, dance company, architectural firm, etc.)." ;
                               rdfs:label "artistic collective type" .


###  https://wendang-project.github.io/ontology/artwork-type
write:artwork-type rdf:type owl:ObjectProperty ;
                   rdfs:domain wd:Q4502142 ,
                               write:TraditionalArtwork ;
                   rdfs:range owl:Thing ;
                   rdfs:comment "Indicates the type of the artwork (e.g., calligraphic work, installation, print, etc.)." ;
                   rdfs:label "artwork type" .


###  http://www.wikidata.org/prop/P50
wdt:P50 rdf:type owl:ObjectProperty ;
        rdfs:domain wd:Q7725634 ;
        rdfs:range owl:Thing ;
        rdfs:comment "Main creator of a written work." ;
        rdfs:label "author" .


###  https://wendang-project.github.io/ontology/background-color
write:background-color rdf:type owl:ObjectProperty ;
                       rdfs:domain write:CalliWritingUnit ;
                       rdfs:range owl:Thing ;
                       rdfs:comment "Background color(s) of the Calli-Writing Unit." ;
                       rdfs:label "background color" .


###  http://www.wikidata.org/prop/P144
wdt:P144 rdf:type owl:ObjectProperty ;
         rdfs:domain write:CalliWritingUnit ;
         rdfs:range owl:Thing ,
                    wd:Q7725634 ;
         rdfs:comment "Literary work on which the Calli-Writing unit is based." ;
         rdfs:label "based on" .


###  https://wendang-project.github.io/ontology/calligrapher
write:calligrapher rdf:type owl:ObjectProperty ;
                   rdfs:domain wd:Q184485 ;
                   rdfs:range wd:Q215627 ;
                   rdfs:comment "Calligrapher who participates in a performing arts event (e.g., performance, musicalligraphy, etc.)." ;
                   rdfs:label "calligrapher" .


###  https://wendang-project.github.io/ontology/character-form
write:character-form rdf:type owl:ObjectProperty ;
                     rdfs:domain write:CalliWritingUnit ;
                     rdfs:range owl:Thing ;
                     rdfs:comment "Form of the Chinese character present in a Calli-Writing unit." ;
                     rdfs:label "character form" .


###  https://wendang-project.github.io/ontology/chinese-concept
write:chinese-concept rdf:type owl:ObjectProperty ;
                      rdfs:domain wd:Q17514 ,
                                  wd:Q184485 ,
                                  write:DecorativeAndAppliedArt ;
                      rdfs:range skos:Concept ;
                      rdfs:comment "Philosophical, literary, cultural, social or other concept or notion represented within the artwork." ;
                      rdfs:label "Chinese concept" .


###  https://wendang-project.github.io/ontology/chinese-visual-element
write:chinese-visual-element rdf:type owl:ObjectProperty ;
                             rdfs:domain wd:Q17514 ,
                                         wd:Q184485 ,
                                         write:DecorativeAndAppliedArt ;
                             rdfs:range skos:Concept ;
                             rdfs:comment "Visual element or motif derived from Chinese culture that appears in the artwork." ;
                             rdfs:label "Chinese visual element" .

###  http://www.wikidata.org/prop/P462
wdt:P462 rdf:type owl:ObjectProperty ;
         rdfs:domain wd:Q17514 ,
                     wd:Q4502142 ,
                     write:CalliWritingUnit ,
                     write:DecorativeAndAppliedArt ;
         rdfs:range owl:Thing ;
         rdfs:comment "Color(s) used in the making of an artwork or a Calli-Writing unit (for the latter, not to be confused with 'write:background-color')." ;
         rdfs:label "color" .


###  http://www.wikidata.org/prop/P88
wdt:P88 rdf:type owl:ObjectProperty ;
        rdfs:domain wd:Q17514 ,
                    wd:Q4502142 ,
                    write:DecorativeAndAppliedArt ;
        rdfs:range owl:Thing ,
                   wd:Q215627 ;
        rdfs:comment "Commissioner of the artwork (person or organisation)." ;
        rdfs:label "commissioned by" .


###  http://www.wikidata.org/prop/P86
wdt:P86 rdf:type owl:ObjectProperty ;
        rdfs:domain wd:Q184485 ;
        rdfs:range wd:Q215627 ;
        rdfs:comment "Person who composed the music for the performing arts event." ;
        rdfs:label "composer" .


###  http://www.wikidata.org/prop/P27
wdt:P27 rdf:type owl:ObjectProperty ;
        rdfs:domain wd:Q215627 ;
        rdfs:range owl:Thing ;
        rdfs:comment "Country of citizenship of the person." ;
        rdfs:label "country of citizenship" .


###  http://www.wikidata.org/prop/P170
wdt:P170 rdf:type owl:ObjectProperty ;
         rdfs:domain wd:Q17514 ,
                     wd:Q4502142 ,
                     wd:Q7725310 ,
                     write:TraditionalArtwork ;
         rdfs:range wd:Q1400264 ,
                    wd:Q215627 ;
         rdfs:comment "Person or artistic collective that created the artwork." ;
         rdfs:label "creator" .


###  https://wendang-project.github.io/ontology/creates-artwork
write:creates-artwork rdf:type owl:ObjectProperty ;
                      rdfs:domain wd:Q184485 ;
                      rdfs:range wd:Q4502142 ;
                      rdfs:comment "Artwork created during a performing arts event (distinct from 'uses artwork')." ;
                      rdfs:label "creates artwork" .


###  http://www.wikidata.org/prop/P1640
wdt:P1640 rdf:type owl:ObjectProperty ;
          rdfs:domain wd:Q464980 ;
          rdfs:range owl:Thing ,
                     wd:Q215627 ;
          rdfs:comment "Person responsible for curating the exhibition." ;
          rdfs:label "curator" .


###  http://www.wikidata.org/prop/P180
wdt:P180 rdf:type owl:ObjectProperty ;
         rdfs:domain write:CalliWritingUnit ,
                     write:WRITEcollections ;
         rdfs:range owl:Thing ;
         rdfs:comment "Subject, theme, or entity visually and / or conceptually expressed in an artwork or a Calli-Writing unit." ;
         rdfs:label "depicts" .


###  http://www.wikidata.org/prop/P287
wdt:P287 rdf:type owl:ObjectProperty ;
         rdfs:domain write:DecorativeAndAppliedArt ;
         rdfs:range wd:Q1400264 ,
                    wd:Q215627 ;
         rdfs:comment "Person or artistic collective responsible for designing a piece of decorative and applied art." ;
         rdfs:label "designer" .


###  http://www.wikidata.org/prop/P10661
wdt:P10661 rdf:type owl:ObjectProperty ;
           rdfs:domain wd:Q464980 ;
           rdfs:range wd:Q215627 ;
           rdfs:comment "Artist(s) whose artworks are displayed in the exhibition." ;
           rdfs:label "exhibited artist" .


###  https://wendang-project.github.io/ontology/exhibited-artwork
write:exhibited-artwork rdf:type owl:ObjectProperty ;
                        rdfs:domain wd:Q464980 ;
                        rdfs:range wd:Q184485 ,
                                   wd:Q4502142 ,
                                   wd:Q7725310 ,
                                   write:DecorativeAndAppliedArt ;
                        rdfs:comment "Artwork(s) displayed in the exhibition." ;
                        rdfs:label "exhibited artwork" .


###  http://www.wikidata.org/prop/P608
wdt:P608 rdf:type owl:ObjectProperty ;
         rdfs:domain wd:Q184485 ,
                     wd:Q4502142 ,
                     write:DecorativeAndAppliedArt ;
         rdfs:range wd:Q464980 ;
         rdfs:comment "Exhibition(s) where an artwork or series of artworks was exhibited." ;
         rdfs:label "exhibition history" .


###  https://www.wikidata.org/prop/P812
<https://www.wikidata.org/prop/P812> rdf:type owl:ObjectProperty ;
                                     rdfs:domain wd:Q215627 ;
                                     rdfs:range owl:Thing ;
                                     rdfs:comment "Academic field of study of the person. Specify only subjects related to the field of arts, without indicating the degree obtained." ;
                                     rdfs:label "field of study" .


###  http://www.wikidata.org/prop/P21
wdt:P21 rdf:type owl:ObjectProperty ;
        rdfs:domain wd:Q215627 ;
        rdfs:range owl:Thing ;
        rdfs:comment "Indicates the gender of the person." ;
        rdfs:label "gender" .


###  http://www.wikidata.org/prop/P136
wdt:P136 rdf:type owl:ObjectProperty ;
         rdfs:domain wd:Q17514 ;
         rdfs:range skos:Concept ;
         rdfs:comment "Provides the classification of a graffiti piece by genre." ;
         rdfs:label "graffiti genre" .


###  https://wendang-project.github.io/ontology/graffiti-style
write:graffiti-style rdf:type owl:ObjectProperty ;
                     rdfs:domain wd:Q17514 ;
                     rdfs:range skos:Concept ;
                     rdfs:comment "Indicates the visual style applied in the creation of a graffiti artwork." ;
                     rdfs:label "graffiti style" .


###  https://wendang-project.github.io/ontology/graffiti-type
write:graffiti-type rdf:type owl:ObjectProperty ;
                    rdfs:domain wd:Q17514 ;
                    rdfs:range skos:Concept ;
                    rdfs:comment "Indicates a specific type or category of graffiti, defined by its form or medium." ;
                    rdfs:label "graffiti type" .


###  http://www.wikidata.org/prop/P527
wdt:P527 rdf:type owl:ObjectProperty ;
         rdfs:domain wd:Q1400264 ,
                     wd:Q43229 ;
         rdfs:range wd:Q215627 ;
         rdfs:comment "Individual(s) who are members of an artistic collective or organisation." ;
         rdfs:label "has member" .


###  https://wendang-project.github.io/ontology/has-unit
write:has-unit rdf:type owl:ObjectProperty ;
               rdfs:domain write:WRITEcollections ;
               rdfs:range write:CalliWritingUnit ;
               rdfs:comment "Links an artwork to its corresponding Calli-Writing unit(s)." ;
               rdfs:label "has unit" .

###  http://www.wikidata.org/prop/P941
wdt:P941 rdf:type owl:ObjectProperty ;
         rdfs:domain wd:Q17514 ,
                     wd:Q184485 ,
                     wd:Q4502142 ;
         rdfs:range owl:Thing ,
                    wd:Q7725634 ;
         rdfs:comment "Object or entity that inspired the creative, artistic work (e.g., literary work, human, place, event)." ;
         rdfs:label "inspired by" .


###  http://www.wikidata.org/prop/P1303
wdt:P1303 rdf:type owl:ObjectProperty ;
          rdfs:domain wd:Q184485 ;
          rdfs:range owl:Thing ;
          rdfs:comment "Musical instrument(s) used during a performing arts event." ;
          rdfs:label "instrument" .        


###  http://www.wikidata.org/prop/P407
wdt:P407 rdf:type owl:ObjectProperty ;
         rdfs:domain write:CalliWritingUnit ;
         rdfs:range owl:Thing ;
         rdfs:comment "Language(s) used in the creation of a Calli-Writing unit." ;
         rdfs:label "language" .


###  http://www.wikidata.org/prop/P276
wdt:P276 rdf:type owl:ObjectProperty ;
         rdfs:domain wd:Q1400264 ,
                     wd:Q17514 ,
                     wd:Q184485 ,
                     wd:Q43229 ,
                     wd:Q464980 ;
         rdfs:range owl:Thing ;
         rdfs:comment "Indicates a specific geographical location (such as a building, city, or country) where an event took place, an artwork is located, or an organisation / artistic collective is based." ;
         rdfs:label "location" .


###  http://www.wikidata.org/prop/P1071
wdt:P1071 rdf:type owl:ObjectProperty ;
          rdfs:domain wd:Q4502142 ,
                      wd:Q7725310 ,
                      write:DecorativeAndAppliedArt ;
          rdfs:range owl:Thing ;
          rdfs:comment "Indicates the city or country where a specific artwork was created." ;
          rdfs:label "location of creation" .


###  http://www.wikidata.org/prop/P176
wdt:P176 rdf:type owl:ObjectProperty ;
         rdfs:domain write:DecorativeAndAppliedArt ;
         rdfs:range owl:Thing ;
         rdfs:comment "Manufacturer or producer of a decorative and applied arts piece." ;
         rdfs:label "manufacturer" .


###  http://www.wikidata.org/prop/P186
wdt:P186 rdf:type owl:ObjectProperty ;
         rdfs:domain write:CalliWritingUnit ,
                     write:WRITEcollections ;
         rdfs:range owl:Thing ;
         rdfs:comment "Material(s) used for creating an artwork, including both primary materials (e.g., ink, paint, clay, stencils) and supporting surfaces (e.g., paper, canvas, wall, train, human body)." ;
         rdfs:label "material" .


###  http://www.wikidata.org/prop/P103
wdt:P103 rdf:type owl:ObjectProperty ;
         rdfs:domain wd:Q215627 ;
         rdfs:range owl:Thing ;
         rdfs:comment "Native language(s) of the person (n.b.: for languages other than native, use 'other language')." ;
         rdfs:label "native language" .


###  http://www.wikidata.org/prop/P106
wdt:P106 rdf:type owl:ObjectProperty ;
         rdfs:domain wd:Q215627 ;
         rdfs:range owl:Thing ;
         rdfs:comment "Work or profession in which a person is engaged." ;
         rdfs:label "occupation" .


###  https://wendang-project.github.io/ontology/organisation-type
write:organisation-type rdf:type owl:ObjectProperty ;
                        rdfs:domain wd:Q43229 ;
                        rdfs:range owl:Thing ;
                        rdfs:comment "Provides the classification of an organisation." ;
                        rdfs:label "organisation type" .


###  http://www.wikidata.org/prop/P664
wdt:P664 rdf:type owl:ObjectProperty ;
         rdfs:domain wd:Q184485 ,
                     wd:Q464980 ;
         rdfs:range wd:Q1400264 ,
                    wd:Q215627 ,
                    wd:Q43229 ;
         rdfs:comment "Person or organisation responsible for organising an event (e.g., exhibition, performing arts event)." ;
         rdfs:label "organiser" .


###  http://www.wikidata.org/prop/P1412
wdt:P1412 rdf:type owl:ObjectProperty ;
          rdfs:domain wd:Q215627 ;
          rdfs:range owl:Thing ;
          rdfs:comment "Language(s) that the person speaks, writes or signes (n.b.: for native language(s), use 'native language')." ;
          rdfs:label "other language" .


###  https://wendang-project.github.io/ontology/other-visual-element
write:visual-element rdf:type owl:ObjectProperty ;
                     rdfs:domain wd:Q17514 ,
                                 write:DecorativeAndAppliedArt ;
                     rdfs:range owl:Thing ;
                     rdfs:comment "Non-Chinese visual element (motif) that appears in the artwork." ;
                     rdfs:label "other visual element" .


###  https://www.wikidata.org/prop/P179
<https://www.wikidata.org/prop/P179> rdf:type owl:ObjectProperty ;
                                     rdfs:domain write:WRITEcollections ;
                                     rdfs:range wd:Q7725310 ;
                                     rdfs:comment "Connects the artwork to the series it belongs to." ;
                                     rdfs:label "part of series" .


###  http://www.wikidata.org/prop/P175
wdt:P175 rdf:type owl:ObjectProperty ;
         rdfs:domain wd:Q184485 ;
         rdfs:range wd:Q1400264 ,
                    wd:Q215627 ;
         rdfs:comment "Person or artistic collective who took part in a performing arts event as a performer, including roles such as dancer, musician, singer, or actor." ;
         rdfs:label "performer" .


###  https://wendang-project.github.io/ontology/performing-art-type
write:performing-art-type rdf:type owl:ObjectProperty ;
                          rdfs:domain wd:Q184485 ;
                          rdfs:range skos:Concept ;
                          rdfs:comment "Indicates the specific type or genre of a performing art." ;
                          rdfs:label "performing art type" .


###  http://www.wikidata.org/prop/P19
wdt:P19 rdf:type owl:ObjectProperty ;
        rdfs:domain wd:Q215627 ;
        rdfs:range owl:Thing ;
        rdfs:comment "Place of birth of the person." ;
        rdfs:label "place of birth" .


###  http://www.wikidata.org/prop/P20
wdt:P20 rdf:type owl:ObjectProperty ;
        rdfs:domain wd:Q215627 ;
        rdfs:range owl:Thing ;
        rdfs:comment "Place of death of the person." ;
        rdfs:label "place of death" .


###  https://wendang-project.github.io/ontology/product-type
write:product-type rdf:type owl:ObjectProperty ;
                   rdfs:domain write:DecorativeAndAppliedArt ;
                   rdfs:range owl:Thing ;
                   rdfs:comment "Indicates the typology of a decorative and applied arts piece." ;
                   rdfs:label "product type" .


###  https://wendang-project.github.io/ontology/relevant-activity-location
write:relevant-activity-location rdf:type owl:ObjectProperty ;
                                 rdfs:domain wd:Q215627 ;
                                 rdfs:range owl:Thing ;
                                 rdfs:comment "Relevant place(s) where the person performs his / her activity." ;
                                 rdfs:label "relevant activity location" .


###  http://www.wikidata.org/prop/P127
wdt:P127 rdf:type owl:ObjectProperty ;
         rdfs:domain wd:Q4502142 ;
         rdfs:range wd:Q1400264 ,
                    wd:Q215627 ,
                    wd:Q43229 ;
         rdfs:comment "Person who holds the rights of the artwork." ;
         rdfs:label "right holder" .


###  http://www.wikidata.org/prop/P9302
wdt:P9302 rdf:type owl:ObjectProperty ;
          rdfs:domain write:CalliWritingUnit ;
          rdfs:range skos:Concept ;
          rdfs:comment "Indicates a specific form / style of the Chinese script used in a Calli-Writing unit." ;
          rdfs:label "script style" .


###  https://wendang-project.github.io/ontology/tag-of
write:tag-of rdf:type owl:ObjectProperty ;
             rdfs:domain write:CalliWritingUnit ;
             rdfs:range wd:Q1400264 ,
                        wd:Q215627 ;
             rdfs:comment "Tag that represents a name of the artist / crew or a symbol." ;
             rdfs:label "tag of" .


###  http://www.wikidata.org/prop/P2283
wdt:P2283 rdf:type owl:ObjectProperty ;
          rdfs:domain write:CalliWritingUnit ,
                      write:WRITEcollections ;
          rdfs:range owl:Thing ;
          rdfs:comment "Tool(s) employed in the creation of the artwork (n.b.: for materials, use 'material')." ;
          rdfs:label "tool" .


###  https://wendang-project.github.io/ontology/uses-artwork
write:uses-artwork rdf:type owl:ObjectProperty ;
                   rdfs:domain wd:Q184485 ,
                               wd:Q4502142 ;
                   rdfs:range wd:Q4502142 ;
                   rdfs:comment "An already-existing artwork incorporated into a performing arts event or used in the creation of another artwork (n.b.: for new artworks produced during a performing arts event, use 'creates artwork')." ;
                   rdfs:label "uses artwork" .


###  https://wendang-project.github.io/ontology/wikidata-resource
write:wikidata-resource rdf:type owl:ObjectProperty ;
                        rdfs:domain wd:Q1400264 ,
                                    wd:Q215627 ,
                                    wd:Q43229 ,
                                    wd:Q464980 ,
                                    wd:Q7725310 ,
                                    wd:Q7725634 ,
                                    write:TraditionalArtwork ,
                                    write:WRITEcollections ;
                        rdfs:range owl:Thing ;
                        rdfs:comment "Wikidata resource which identifies the record." ;
                        rdfs:label "wikidata resource" .


###  https://www.wikidata.org/prop/P282
<https://www.wikidata.org/prop/P282> rdf:type owl:ObjectProperty ;
                                     rdfs:domain write:CalliWritingUnit ;
                                     rdfs:range owl:Thing ;
                                     rdfs:comment "Characters, alphabet or other system of writing used in a Calli-Writing unit." ;
                                     rdfs:label "writing system" .


#################################################################
#    Data properties
#################################################################

###  http://www.wikidata.org/prop/P1480
wdt:P1480 rdf:type owl:DatatypeProperty ;
          rdfs:domain wd:Q7725634 ,
                      write:CalliWritingUnit ;
          rdfs:range xsd:string ;
          rdfs:comment "Accuracy indicator for character count in the Calli-Writing unit and date of creation of the literary work (allowed value: 'circa')." ;
          rdfs:label "accuracy" .


###  https://wendang-project.github.io/ontology/attributed-title
write:attributed-title rdf:type owl:DatatypeProperty ;
                      rdfs:domain write:CalliWritingUnit ;
                      rdfs:range xsd:string ;
                      rdfs:comment "Title attributed to the Calli-Writing unit (to use without language tag)." ;
                      rdfs:label "attributed title" .


###  https://wendang-project.github.io/ontology/big-characters-calligraphy
write:big-characters-calligraphy rdf:type owl:DatatypeProperty ;
                                 rdfs:domain write:CalliWritingUnit ;
                                 rdfs:range xsd:string ;
                                 rdfs:comment "Indicates the presence or absence of big calligraphic characters in the Calli-Writing unit (allowed values: 'Present', 'Not present')." ;
                                 rdfs:label "big characters calligraphy" .


###  https://wendang-project.github.io/ontology/calligraphic-line
write:calligraphic-line rdf:type owl:DatatypeProperty ;
                        rdfs:domain write:CalliWritingUnit ;
                        rdfs:range xsd:string ;
                        rdfs:comment "Indicates the presence or absence of a calligraphic line within a Calli-Writing unit (allowed values: 'Present', 'Not present')." ;
                        rdfs:label "calligraphic line" .


###  https://wendang-project.github.io/ontology/calligraphic-training
write:calligraphic-training rdf:type owl:DatatypeProperty ;
                             rdfs:domain wd:Q215627 ;
                             rdfs:range xsd:string ;
                             rdfs:comment "Indicates the type of calligraphic education the person has (allowed values: 'Familial', 'Self-Taught', 'Academic', 'School', 'Not present', 'Present (not specified)')." ;
                             rdfs:label "calligraphic training" .


###  http://www.wikidata.org/prop/P585
wdt:P585 rdf:type owl:DatatypeProperty ;
         rdfs:domain wd:Q184485 ;
         rdfs:range xsd:date ;
         rdfs:comment "Date in which a performing arts event occurred." ;
         rdfs:label "date" .


###  http://www.wikidata.org/prop/P569
wdt:P569 rdf:type owl:DatatypeProperty ;
         rdfs:domain wd:Q215627 ;
         rdfs:range xsd:date ;
         rdfs:comment "Date of birth of the person." ;
         rdfs:label "date of birth" .

###  http://www.wikidata.org/prop/P571
wdt:P571 rdf:type owl:DatatypeProperty ;
         rdfs:domain wd:Q1400264 ,
                     wd:Q17514 ,
                     wd:Q43229 ,
                     wd:Q4502142 ,
                     wd:Q7725634 ,
                     write:DecorativeAndAppliedArt ,
                     write:TraditionalArtwork ;
         rdfs:range xsd:date ;
         rdfs:comment "Date when the artwork, the literary work, the artistic collective or the organisation was created (n.b.: for performing arts, use 'date')." ;
         rdfs:label "date of creation" .


###  http://www.wikidata.org/prop/P570
wdt:P570 rdf:type owl:DatatypeProperty ;
         rdfs:domain wd:Q215627 ;
         rdfs:range xsd:date ;
         rdfs:comment "Date of death of the person." ;
         rdfs:label "date of death" .


###  http://www.wikidata.org/prop/P973
wdt:P973 rdf:type owl:DatatypeProperty ;
         rdfs:range xsd:anyURI ;
         rdfs:comment "Link to the website where the resource is described." ;
         rdfs:label "described at URL" .


###  http://www.wikidata.org/prop/P1343
wdt:P1343 rdf:type owl:DatatypeProperty ;
          rdfs:range xsd:string ;
          rdfs:comment "Bibliographic source(s) of the resource." ;
          rdfs:label "described by source" .


###  https://wendang-project.github.io/ontology/description
write:description rdf:type owl:DatatypeProperty ;
                  rdfs:range xsd:string ;
                  rdfs:comment "Textual description of the resource." ;
                  rdfs:label "description" .


###  https://www.wikidata.org/prop/P1406
<https://www.wikidata.org/prop/P1406> rdf:type owl:DatatypeProperty ;
                                               rdfs:domain write:CalliWritingUnit ;
                                               rdfs:range xsd:string ;
                                               rdfs:comment "Direction of the writing within a Calli-Writing unit (allowed values: 'Traditional', 'Modern', 'Free', 'Unidentifiable')." ;
                                               rdfs:label "directionality" .


###  http://www.wikidata.org/prop/P2047
wdt:P2047 rdf:type owl:DatatypeProperty ;
          rdfs:domain wd:Q184485 ;
          rdfs:range xsd:duration ;
          rdfs:comment "Duration of the performing arts event." ;
          rdfs:label "duration" .


###  http://www.wikidata.org/prop/P582
wdt:P582 rdf:type owl:DatatypeProperty ;
         rdfs:domain wd:Q464980 ,
                     wd:Q7725310 ;
         rdfs:range xsd:date ;
         rdfs:comment "Date when the event finished." ;
         rdfs:label "end time" .


###  https://wendang-project.github.io/ontology/has-chengyu
write:has-chengyu rdf:type owl:DatatypeProperty ;
                  rdfs:domain wd:Q17514 ;
                  rdfs:range xsd:string ;
                  rdfs:comment "Indicates the presence or absence of the four-character traditional Chinese idiomatic expression (allowed values: 'Yes', 'No')." ;
                  rdfs:label "has chengyu" .


###  http://www.wikidata.org/prop/P8570
wdt:P8570 rdf:type owl:DatatypeProperty ;
          rdfs:domain wd:Q17514 ,
                      wd:Q4502142 ,
                      write:CalliWritingUnit ,
                      write:DecorativeAndAppliedArt ;
          rdfs:range xsd:string ;
          rdfs:comment "Indicates the presence or absence of a colophon, which typically includes the time or date when the artwork was completed, the name of the artist, and the location (allowed values: 'Yes', 'No')." ;
          rdfs:label "has colophon" .


###  https://wendang-project.github.io/ontology/has-seal
write:has-seal rdf:type owl:DatatypeProperty ;
               rdfs:domain wd:Q17514 ,
                           wd:Q4502142 ,
                           write:DecorativeAndAppliedArt ,
                           write:TraditionalArtwork ;
               rdfs:range xsd:string ;
               rdfs:comment "Indicates the presence or absence of a seal, typically square-shaped and red-coloured, which serves as the signature of the artist (allowed values: 'Yes', 'No')." ;
               rdfs:label "has seal" .


###  http://www.wikidata.org/prop/P2048
wdt:P2048 rdf:type owl:DatatypeProperty ;
          rdfs:domain wd:Q17514 ,
                      wd:Q4502142 ,
                      write:DecorativeAndAppliedArt ;
          rdfs:range xsd:string ;
          rdfs:comment "Height of the artwork." ;
          rdfs:label "height" .


###  http://www.wikidata.org/prop/P2561
wdt:P2561 rdf:type owl:DatatypeProperty ;
          rdfs:domain wd:Q1400264 ,
                      wd:Q215627 ,
                      wd:Q43229 ;
          rdfs:range xsd:string ;
          rdfs:comment "Name of the person, artistic collective, or organisation. For a person, provide the name and surname without a language tag. For an artistic collective or organisation, provide the name in @en, @zh-Latn, and @zh, if applicable." ;
          rdfs:label "name" .


###  https://wendang-project.github.io/ontology/note
write:note rdf:type owl:DatatypeProperty ;
           rdfs:range xsd:string ;
           rdfs:comment "Notes of any kind related to the item (private use only)." ;
           rdfs:label "notes" .


###  https://wendang-project.github.io/ontology/number-of-characters
write:number-of-characters rdf:type owl:DatatypeProperty ;
                           rdfs:domain write:CalliWritingUnit ;
                           rdfs:range xsd:integer ;
                           rdfs:comment "Number of Chinese characters in a Calli-Writing unit." ;
                           rdfs:label "number of characters" .


###  http://www.wikidata.org/prop/P856
wdt:P856 rdf:type owl:DatatypeProperty ;
         rdfs:domain wd:Q1400264 ,
                     wd:Q184485 ,
                     wd:Q215627 ,
                     wd:Q43229 ,
                     wd:Q4502142 ,
                     wd:Q464980 ,
                     write:DecorativeAndAppliedArt ;
         rdfs:range xsd:anyURI ;
         rdfs:comment "Link to the official website of the resource." ;
         rdfs:label "official website" .


###  http://www.wikidata.org/prop/P2284
wdt:P2284 rdf:type owl:DatatypeProperty ;
          rdfs:domain write:DecorativeAndAppliedArt ;
          rdfs:range xsd:string ;
          rdfs:comment "Published price listed or paid for the artwork, to be complemented with the currency (e.g., 100 EUR)." ;
          rdfs:label "price" .


###  http://www.wikidata.org/prop/P742
wdt:P742 rdf:type owl:DatatypeProperty ;
         rdfs:domain wd:Q215627 ;
         rdfs:range xsd:string ;
         rdfs:comment "Pseudonym of the person (n.b.: the same rules for the 'name' apply)." ;
         rdfs:label "pseudonym" .


###  https://wendang-project.github.io/ontology/significance
write:significance rdf:type owl:DatatypeProperty ;
                   rdfs:domain write:CalliWritingUnit ;
                   rdfs:range xsd:string ;
                   rdfs:comment "Indicates whether the content of a Calli-Writing unit is meaningful, meaningless, or illegible (allowed values: 'Meaningful writing', 'Set of lines (meaningless)', 'Set of signs (illegible)')." ;
                   rdfs:label "significance" .


###  http://www.wikidata.org/prop/P580
wdt:P580 rdf:type owl:DatatypeProperty ;
         rdfs:domain wd:Q464980 ,
                     wd:Q7725310 ;
         rdfs:range xsd:date ;
         rdfs:comment "Date when the event started." ;
         rdfs:label "start time" .


###  http://www.wikidata.org/prop/P6375
wdt:P6375 rdf:type owl:DatatypeProperty ;
          rdfs:domain wd:Q17514 ;
          rdfs:range xsd:string ;
          rdfs:comment "Street address where the graffiti piece was created (include any relevant location details)." ;
          rdfs:label "street address" .


###  https://wendang-project.github.io/ontology/tag
write:tag rdf:type owl:DatatypeProperty ;
          rdfs:domain wd:Q215627 ;
          rdfs:range xsd:string ;
          rdfs:comment "Signature of the graffiti writer (n.b.: multiple values are possible, each accompanied by a language tag)." ;
          rdfs:label "tag" .


###  http://www.wikidata.org/prop/P1476
wdt:P1476 rdf:type owl:DatatypeProperty ;
          rdfs:domain wd:Q464980 ,
                      wd:Q7725310 ,
                      wd:Q7725634 ,
                      write:TraditionalArtwork ,
                      write:WRITEcollections ;
          rdfs:range xsd:string ;
          rdfs:comment "Title of the artwork, literary work, exhibition, or series of creative works (n.b.: multiple values are possible, each accompanied by a language tag)." ;
          rdfs:label "title" .


###  https://wendang-project.github.io/ontology/transcription-and-translation
write:transcription-and-translation rdf:type owl:DatatypeProperty ;
                                  rdfs:domain wd:Q7725634 ,
                                              write:CalliWritingUnit ;
                                  rdfs:range xsd:string ;
                                  rdfs:comment "Transcription and translation of the content of a Calli-Writing unit or (a section of) a literary work (n.b.: multiple values are possible, each accompanied by a language tag)." ;
                                  rdfs:label "transcription and translation" .


###  https://wendang-project.github.io/ontology/vectorised-digitised-artwork
write:vectorised-digitised-artwork rdf:type owl:DatatypeProperty ;
                                   rdfs:domain wd:Q4502142 ,
                                               write:CalliWritingUnit ;
                                   rdfs:range xsd:string ;
                                   rdfs:comment "Indicates whether the artwork or the Calli-Writing unit have been vectorised or digitised (allowed value: 'Yes')." ;
                                   rdfs:label "vectorised or digitised" .


###  http://www.wikidata.org/prop/P2049
wdt:P2049 rdf:type owl:DatatypeProperty ;
          rdfs:domain wd:Q17514 ,
                      wd:Q4502142 ,
                      write:DecorativeAndAppliedArt ;
          rdfs:range xsd:string ;
          rdfs:comment "Width of the artwork." ;
          rdfs:label "width" .

#################################################################
#    Classes
#################################################################

###  http://www.w3.org/2004/02/skos/core#Concept
skos:Concept rdf:type owl:Class .


###  http://www.wikidata.org/entity/Q1400264
wd:Q1400264 rdf:type owl:Class ;
            rdfs:comment "Group of artists from diverse disciplines (e.g., calligraphers, graffiti writers, dancers, etc.) collaborating to create collective artistic works of any kind." ;
            rdfs:label "Artistic Collective" .


###  https://wendang-project.github.io/ontology/CalliWritingUnit
write:CalliWritingUnit rdf:type owl:Class ;
                       rdfs:comment "In an artwork, a content unit featuring elements of calligraphy and / or writing, in a form of meaningful writing, set of signs and / or set of lines." ;
                       rdfs:label "Calli-Writing Unit" .


###  https://wendang-project.github.io/ontology/DecorativeAndAppliedArt
write:DecorativeAndAppliedArt rdf:type owl:Class ;
                              rdfs:subClassOf write:WRITEcollections ;
                              rdfs:comment "A class that includes artworks from the WRITE collection specifically categorised under Decorative and Applied Arts." ;
                              rdfs:label "Decorative and Applied Arts" .


###  http://www.wikidata.org/entity/Q464980
wd:Q464980 rdf:type owl:Class ;
           rdfs:comment "Exhibition showcasing one or more artworks (or artworks' series) from the four WRITE collections." ;
           rdfs:label "Exhibition" .


###  http://www.wikidata.org/entity/Q17514
wd:Q17514 rdf:type owl:Class ;
          rdfs:subClassOf write:WRITEcollections ;
          rdfs:comment "A class that includes artworks from the WRITE collection specifically categorised under Graffiti." ;
          rdfs:label "Graffiti" .


###  http://www.wikidata.org/entity/Q7725634
wd:Q7725634 rdf:type owl:Class ;
            rdfs:comment "Literary work (in whole or in part) that serves as the basis or inspiration for a Calli-Writing unit, or the creation of an artwork." ;
            rdfs:label "Literary Work" .


###  http://www.wikidata.org/entity/Q43229
wd:Q43229 rdf:type owl:Class ;
          rdfs:comment "Organisation involved in the production / commissioning of an artwork or the organisation of an exhibition." ;
          rdfs:label "Organisation" .


###  http://www.wikidata.org/entity/Q184485
wd:Q184485 rdf:type owl:Class ;
           rdfs:subClassOf write:WRITEcollections ;
           rdfs:comment "A class that includes artworks from the WRITE collection specifically categorised under Performing Arts." ;
           rdfs:label "Performing Arts" .


###  http://www.wikidata.org/entity/Q215627
wd:Q215627 rdf:type owl:Class ;
           rdfs:comment "This class represents individuals who engage in creative, artistic, or organisational roles (such as calligraphers, musicians, dancers, singers, graffiti writers, authors, creators, organisers, curators, and others)." ;
           rdfs:label "Person" .


###  http://www.wikidata.org/entity/Q7725310
wd:Q7725310 rdf:type owl:Class ;
            rdfs:comment "Class that represents a set of related artworks that might be included in the four WRITE collections." ;
            rdfs:label "Series of Creative Works" .


###  https://wendang-project.github.io/ontology/TraditionalArtwork
write:TraditionalArtwork rdf:type owl:Class ;
                         rdfs:comment "Artwork that follows traditional calligraphic canons and / or is created before 1980. This artwork does not belong to any of the four WRITE collections, but it is somehow related to one or more artworks from these collections." ;
                         rdfs:label "Traditional Artwork" .


###  http://www.wikidata.org/entity/Q4502142
wd:Q4502142 rdf:type owl:Class ;
            rdfs:subClassOf write:WRITEcollections ;
            rdfs:comment "A class that includes artworks from the WRITE collection specifically categorised under Visual Arts." ;
            rdfs:label "Visual Arts" .


###  https://wendang-project.github.io/ontology/WRITEcollections
write:WRITEcollections rdf:type owl:Class ;
                       rdfs:comment "The superclass that encompasses artworks from four distinct types of art (Decorative and Applied Arts, Graffiti, Performing Arts and Visual Arts). There are four WRITE collections, one for each art category." ;
                       rdfs:label "WRITE collections" .


###  Generated by the OWL API (version 4.5.29.2024-05-13T12:11:03Z) https://github.com/owlcs/owlapi
